remove name from implies, update proplang drivers

experiments/coq-experiments/proplang/EnergyComparison/Analysis.py
@@ -223,6 +223,12 @@ def analyze(results: str, images: str):
             show=False,
         )
 
+    df['throughput'] = (df['inputs'] + df['discards']) / df['time']
+
+    # Calculate the mean throughput for each workload and strategy
+    df = df.groupby(['workload', 'strategy', 'version']).mean().reset_index()
+    df.to_csv(f'{images}/mean.csv')
+
 if __name__ == "__main__":
 
     filepath = pathlib.Path(__file__).resolve().parent
