experiments/coq-experiments/proplang/EnergyComparison/Collect.py
@@ -19,7 +19,6 @@ def collect(results: str):
 
         tool._preprocess(workload)
 
-
         for mixture in mixtures:
             print("Mixture")
             for variable, version  in mixture:
@@ -38,20 +37,12 @@ def collect(results: str):
                         continue
 
                     for property in tool.all_properties(workload):
-                        if workload.name.startswith('STLC'):
-                            property = 'test_' + property + '_runner'
-                            pass
-                        elif workload.name.endswith('Proplang'):
-                            property = 'test_' + property + '_runner'
-                            if property[10:-7] not in tasks[workload.name[:3]][variant.name]:
-                                print(f'Skipping {workload.name},{strategy.name},{variant.name},{property}')
-                                continue
-                        elif workload.name == 'BST':
-                            property = 'test_' + property
-                            if property[10:] not in tasks["BST"][variant.name]:
-                                print(f'Skipping {workload.name},{strategy.name},{variant.name},{property}')
-                                continue
-                        
+                        property = 'test_' + property
+                        workloadname = workload.name if not workload.name.endswith('Proplang') else workload.name[:-8]
+                        if property[10:] not in tasks[workloadname][variant.name]:
+                            print(f'Skipping {workload.name},{strategy.name},{variant.name},{property}')
+                            continue
+                    
                         # Don't compile tasks that are already completed.
                         finished = set(os.listdir(results))
                         file = f'{workload.name},{strategy.name},{variable.current},{variant.name},{property}'
