workloads/Coq/BSTProplang/Strategies/TypeBasedFuzzer.v
@@ -18,15 +18,6 @@ Local Open Scope prop_scope.
 
 Derive (Arbitrary, Show, Sized, Fuzzy) for Tree.
 
-#[local] Instance FuzzyProd {A} `{Fuzzy A} {B} `{Fuzzy B}  : Fuzzy (A * B)  :=
-{|
-  fuzz ab :=
-    (let '(a, b) := ab in
-    ma <- fuzz a ;;
-    mb <- fuzz b ;;
-    ret (ma,mb))
-|}.
-
 #[local] Instance dec_eq_tree : Dec_Eq Tree.
 Proof. dec_eq. Defined.
 
@@ -34,8 +25,8 @@ Axiom number_of_trials : nat.
 Extract Constant number_of_trials => "max_int".
 
 Definition prop_InsertValid   :=
-	ForAll "t" (fun tt => arbitrary) (fun tt t => fuzz t) (fun tt => shrink) (fun tt => show) (
-	Implies (Tree · ∅) "isBST t" (fun '(t, tt) => isBST t) (
+	ForAll "t" (fun tt => arbitrary) (fun tt => fuzz) (fun tt => shrink) (fun tt => show) (
+	Implies (Tree · ∅) (fun '(t, tt) => isBST t) (
 	ForAll "k" (fun tt => arbitrary) (fun tt k => arbitrary) (fun tt => shrink) (fun tt => show) (
 	ForAll "v" (fun tt => arbitrary) (fun tt v => arbitrary) (fun tt => shrink) (fun tt => show) (
 	Check (nat · (nat · (Tree · ∅)))
@@ -45,8 +36,8 @@ Definition test_prop_InsertValid := (fuzzLoop number_of_trials prop_InsertValid 
 (*! QuickProp test_prop_InsertValid. *)
 
 Definition prop_DeleteValid   :=
-	ForAll "t" (fun tt => arbitrary) (fun tt t => fuzz t) (fun tt => shrink) (fun tt => show) (
-	Implies (Tree · ∅) "isBST t" (fun '(t, tt) => isBST t) (
+	ForAll "t" (fun tt => arbitrary) (fun tt => fuzz) (fun tt => shrink) (fun tt => show) (
+	Implies (Tree · ∅) (fun '(t, tt) => isBST t) (
 	ForAll "k" (fun tt => arbitrary) (fun tt n => arbitrary) (fun tt => shrink) (fun tt => show) (
 	Check (nat · (Tree · ∅))
 	(fun '(k, (t, tt)) => (isBST (delete k t)))))).
@@ -55,10 +46,10 @@ Definition test_prop_DeleteValid := (fuzzLoop number_of_trials prop_DeleteValid 
 (*! QuickProp test_prop_DeleteValid. *)
 
 Definition prop_UnionValid :=
-	ForAll "t1" (fun tt => arbitrary) (fun tt t => fuzz t) (fun tt => shrink) (fun tt => show) (
-	Implies (Tree · ∅) "isBST t1" (fun '(t1, tt) => isBST t1) (
+	ForAll "t1" (fun tt => arbitrary) (fun tt => fuzz) (fun tt => shrink) (fun tt => show) (
+	Implies (Tree · ∅) (fun '(t1, tt) => isBST t1) (
 	ForAll "t2" (fun tt => arbitrary) (fun tt t2 => fuzz t2) (fun tt => shrink) (fun tt => show) (
-	Implies (Tree · _) "isBST t2" (fun '(t2, _) => isBST t2) (
+	Implies (Tree · _) (fun '(t2, _) => isBST t2) (
 	Check (Tree · (Tree · ∅))
 	(fun '(t2, (t1, tt)) => (isBST (union t1 t2))))))).
 
@@ -66,8 +57,8 @@ Definition test_prop_UnionValid := (fuzzLoop number_of_trials prop_UnionValid (H
 (*! QuickProp test_prop_UnionValid. *)
 
 Definition prop_InsertPost :=
-	ForAll "t" (fun tt => arbitrary) (fun tt t => fuzz t) (fun tt => shrink) (fun tt => show) (
-	Implies (Tree · ∅) "isBST t" (fun '(t, tt) => isBST t) (
+	ForAll "t" (fun tt => arbitrary) (fun tt => fuzz) (fun tt => shrink) (fun tt => show) (
+	Implies (Tree · ∅) (fun '(t, tt) => isBST t) (
 	ForAll "k" (fun tt => arbitrary) (fun tt k => arbitrary) (fun tt => shrink) (fun tt => show) (
 	ForAll "k'" (fun tt => arbitrary) (fun tt k' => arbitrary) (fun tt => shrink) (fun tt => show) (
 	ForAll "v" (fun tt => arbitrary) (fun tt v => arbitrary) (fun tt => shrink) (fun tt => show) (
@@ -79,8 +70,8 @@ Definition test_prop_InsertPost := (fuzzLoop number_of_trials prop_InsertPost (H
 
 
 Definition prop_DeletePost :=
-	ForAll "t" (fun tt => arbitrary) (fun tt t => fuzz t) (fun tt => shrink) (fun tt => show) (
-	Implies (Tree · ∅) "isBST t" (fun '(t, tt) => isBST t) (
+	ForAll "t" (fun tt => arbitrary) (fun tt => fuzz) (fun tt => shrink) (fun tt => show) (
+	Implies (Tree · ∅) (fun '(t, tt) => isBST t) (
 	ForAll "k" (fun tt => arbitrary) (fun tt t => arbitrary) (fun tt => shrink) (fun tt => show) (
 	ForAll "k'" (fun tt => arbitrary) (fun tt n => arbitrary) (fun tt => shrink) (fun tt => show) (
 	Check (nat · (nat · (Tree · ∅)))
@@ -90,9 +81,9 @@ Definition test_prop_DeletePost := (fuzzLoop number_of_trials prop_DeletePost (H
 (*! QuickProp test_prop_DeletePost. *)
 
 Definition prop_UnionPost :=
-	ForAll "t" (fun tt => arbitrary) (fun tt t => fuzz t) (fun tt => shrink) (fun tt => show) (
-	Implies (Tree · ∅) "isBST t" (fun '(t, tt) => isBST t) (
-	ForAll "t'" (fun tt => arbitrary) (fun tt t' => fuzz t') (fun tt => shrink) (fun tt => show) (
+	ForAll "t" (fun tt => arbitrary) (fun tt => fuzz) (fun tt => shrink) (fun tt => show) (
+	Implies (Tree · ∅) (fun '(t, tt) => isBST t) (
+	ForAll "t'" (fun tt => arbitrary) (fun tt => fuzz) (fun tt => shrink) (fun tt => show) (
 	ForAll "k" (fun tt => arbitrary) (fun tt k => arbitrary) (fun tt => shrink) (fun tt => show) (
 	Check (nat · (Tree · (Tree · ∅)))
 	(fun '(k, (t', (t, tt))) => (let lhs := find k (union t t') in
@@ -108,8 +99,8 @@ Definition test_prop_UnionPost := (fuzzLoop number_of_trials prop_UnionPost (Hea
 (*! QuickProp test_prop_UnionPost. *)
 
 Definition prop_InsertModel :=
-	ForAll "t" (fun tt => arbitrary) (fun tt t => fuzz t) (fun tt => shrink) (fun tt => show) (
-	Implies (Tree · ∅) "isBST t" (fun '(t, tt) => isBST t) (
+	ForAll "t" (fun tt => arbitrary) (fun tt => fuzz) (fun tt => shrink) (fun tt => show) (
+	Implies (Tree · ∅) (fun '(t, tt) => isBST t) (
 	ForAll "k" (fun tt => arbitrary) (fun tt t => arbitrary) (fun tt => shrink) (fun tt => show) (
 	ForAll "v" (fun tt => arbitrary) (fun tt n => arbitrary) (fun tt => shrink) (fun tt => show) (
 	Check (nat · (nat · (Tree · ∅)))
@@ -119,8 +110,8 @@ Definition test_prop_InsertModel := (fuzzLoop number_of_trials prop_InsertModel 
 (*! QuickProp test_prop_InsertModel. *)
 
 Definition prop_DeleteModel :=
-	ForAll "t" (fun tt => arbitrary) (fun tt t => fuzz t) (fun tt => shrink) (fun tt => show) (
-	Implies (Tree · ∅) "isBST t" (fun '(t, tt) => isBST t) (
+	ForAll "t" (fun tt => arbitrary) (fun tt => fuzz) (fun tt => shrink) (fun tt => show) (
+	Implies (Tree · ∅) (fun '(t, tt) => isBST t) (
 	ForAll "k" (fun tt => arbitrary) (fun tt t => arbitrary) (fun tt => shrink) (fun tt => show) (
 	Check (nat · (Tree · ∅))
 	(fun '(k, (t, tt)) => ((toList (delete k t) = deleteKey k (toList t))?))))).
@@ -129,10 +120,10 @@ Definition test_prop_DeleteModel := (fuzzLoop number_of_trials prop_DeleteModel 
 (*! QuickProp test_prop_DeleteModel. *)
 
 Definition prop_UnionModel :=
-	ForAll "t" (fun tt => arbitrary) (fun tt t => fuzz t) (fun tt => shrink) (fun tt => show) (
-	Implies (Tree · ∅) "isBST t" (fun '(t, tt) => isBST t) (
-	ForAll "t'" (fun tt => arbitrary) (fun tt t' => fuzz t') (fun tt => shrink) (fun tt => show) (
-	Implies (Tree · _) "isBST t'" (fun '(t', _) => isBST t') (
+	ForAll "t" (fun tt => arbitrary) (fun tt => fuzz) (fun tt => shrink) (fun tt => show) (
+	Implies (Tree · ∅) (fun '(t, tt) => isBST t) (
+	ForAll "t'" (fun tt => arbitrary) (fun tt => fuzz) (fun tt => shrink) (fun tt => show) (
+	Implies (Tree · _) (fun '(t', _) => isBST t') (
 	Check (Tree · (Tree · ∅))
 	(fun '(t', (t, tt)) => ((toList (union t t') = L_sort (L_unionBy (fun x y => x) (toList t) (toList t')))?)))))).
 
@@ -140,8 +131,8 @@ Definition test_prop_UnionModel := (fuzzLoop number_of_trials prop_UnionModel (H
 (*! QuickProp test_prop_UnionModel. *)
 
 Definition prop_InsertInsert :=
-	ForAll "t" (fun tt => arbitrary) (fun tt t => fuzz t) (fun tt => shrink) (fun tt => show) (
-	Implies (Tree · ∅) "isBST t" (fun '(t, tt) => isBST t) (
+	ForAll "t" (fun tt => arbitrary) (fun tt => fuzz) (fun tt => shrink) (fun tt => show) (
+	Implies (Tree · ∅) (fun '(t, tt) => isBST t) (
 	ForAll "k" (fun tt => arbitrary) (fun tt t => arbitrary) (fun tt => shrink) (fun tt => show) (
 	ForAll "k'" (fun tt => arbitrary) (fun tt n => arbitrary) (fun tt => shrink) (fun tt => show) (
 	ForAll "v" (fun tt => arbitrary) (fun tt v => arbitrary) (fun tt => shrink) (fun tt => show) (
@@ -153,8 +144,8 @@ Definition test_prop_InsertInsert := (fuzzLoop number_of_trials prop_InsertInser
 (*! QuickProp test_prop_InsertInsert. *)
 
 Definition prop_InsertDelete :=
-	ForAll "t" (fun tt => arbitrary) (fun tt t => fuzz t) (fun tt => shrink) (fun tt => show) (
-	Implies (Tree · ∅) "isBST t" (fun '(t, tt) => isBST t) (
+	ForAll "t" (fun tt => arbitrary) (fun tt => fuzz) (fun tt => shrink) (fun tt => show) (
+	Implies (Tree · ∅) (fun '(t, tt) => isBST t) (
 	ForAll "k" (fun tt => arbitrary) (fun tt k => arbitrary) (fun tt => shrink) (fun tt => show) (
 	ForAll "k'" (fun tt => arbitrary) (fun tt k' => arbitrary) (fun tt => shrink) (fun tt => show) (
 	ForAll "v" (fun tt => arbitrary) (fun tt v => arbitrary) (fun tt => shrink) (fun tt => show) (
@@ -165,10 +156,10 @@ Definition test_prop_InsertDelete := (fuzzLoop number_of_trials prop_InsertDelet
 (*! QuickProp test_prop_InsertDelete. *)
 
 Definition prop_InsertUnion :=
-	ForAll "t" (fun tt => arbitrary) (fun tt t => fuzz t) (fun tt => shrink) (fun tt => show) (
-	Implies (Tree · ∅) "isBST t" (fun '(t, tt) => isBST t) (
-	ForAll "t'" (fun tt => arbitrary) (fun tt t' => fuzz t') (fun tt => shrink) (fun tt => show) (
-	Implies (Tree · _) "isBST t'" (fun '(t', _) => isBST t') (
+	ForAll "t" (fun tt => arbitrary) (fun tt => fuzz) (fun tt => shrink) (fun tt => show) (
+	Implies (Tree · ∅) (fun '(t, tt) => isBST t) (
+	ForAll "t'" (fun tt => arbitrary) (fun tt => fuzz) (fun tt => shrink) (fun tt => show) (
+	Implies (Tree · _) (fun '(t', _) => isBST t') (
 	ForAll "k" (fun tt => arbitrary) (fun tt k => arbitrary) (fun tt => shrink) (fun tt => show) (
 	ForAll "v" (fun tt => arbitrary) (fun tt v => arbitrary) (fun tt => shrink) (fun tt => show) (
 	Check (nat · (nat · (Tree · (Tree · ∅))))
@@ -178,8 +169,8 @@ Definition test_prop_InsertUnion := (fuzzLoop number_of_trials prop_InsertUnion 
 (*! QuickProp test_prop_InsertUnion. *)
 
 Definition prop_DeleteInsert :=
-	ForAll "t" (fun tt => arbitrary) (fun tt t => fuzz t) (fun tt => shrink) (fun tt => show) (
-	Implies (Tree · ∅) "isBST t" (fun '(t, tt) => isBST t) (
+	ForAll "t" (fun tt => arbitrary) (fun tt => fuzz) (fun tt => shrink) (fun tt => show) (
+	Implies (Tree · ∅) (fun '(t, tt) => isBST t) (
 	ForAll "k" (fun tt => arbitrary) (fun tt t => arbitrary) (fun tt => shrink) (fun tt => show) (
 	ForAll "k'" (fun tt => arbitrary) (fun tt n => arbitrary) (fun tt => shrink) (fun tt => show) (
 	ForAll "v'" (fun tt => arbitrary) (fun tt v => arbitrary) (fun tt => shrink) (fun tt => show) (
@@ -190,8 +181,8 @@ Definition test_prop_DeleteInsert := (fuzzLoop number_of_trials prop_DeleteInser
 (*! QuickProp test_prop_DeleteInsert. *)
 
 Definition prop_DeleteDelete :=
-	ForAll "t" (fun tt => arbitrary) (fun tt t => fuzz t) (fun tt => shrink) (fun tt => show) (
-	Implies (Tree · ∅) "isBST t" (fun '(t, tt) => isBST t) (
+	ForAll "t" (fun tt => arbitrary) (fun tt => fuzz) (fun tt => shrink) (fun tt => show) (
+	Implies (Tree · ∅) (fun '(t, tt) => isBST t) (
 	ForAll "k" (fun tt => arbitrary) (fun tt t => arbitrary) (fun tt => shrink) (fun tt => show) (
 	ForAll "k'" (fun tt => arbitrary) (fun tt n => arbitrary) (fun tt => shrink) (fun tt => show) (
 	Check (nat · (nat · (Tree · ∅)))
@@ -201,10 +192,10 @@ Definition test_prop_DeleteDelete := (fuzzLoop number_of_trials prop_DeleteDelet
 (*! QuickProp test_prop_DeleteDelete. *)
 
 Definition prop_DeleteUnion :=
-	ForAll "t" (fun tt => arbitrary) (fun tt t => fuzz t) (fun tt => shrink) (fun tt => show) (
-	Implies (Tree · ∅) "isBST t" (fun '(t, tt) => isBST t) (
-	ForAll "t'" (fun tt => arbitrary) (fun tt t' => fuzz t') (fun tt => shrink) (fun tt => show) (
-	Implies (Tree · _) "isBST t'" (fun '(t', _) => isBST t') (
+	ForAll "t" (fun tt => arbitrary) (fun tt => fuzz) (fun tt => shrink) (fun tt => show) (
+	Implies (Tree · ∅) (fun '(t, tt) => isBST t) (
+	ForAll "t'" (fun tt => arbitrary) (fun tt => fuzz) (fun tt => shrink) (fun tt => show) (
+	Implies (Tree · _) (fun '(t', _) => isBST t') (
 	ForAll "k" (fun tt => arbitrary) (fun tt k => arbitrary) (fun tt => shrink) (fun tt => show) (
 	Check (nat · (Tree · (Tree · ∅)))
 	(fun '(k, (t', (t, tt))) => (delete k (union t t') =|= union (delete k t) (delete k t')))))))).
@@ -213,10 +204,10 @@ Definition test_prop_DeleteUnion := (fuzzLoop number_of_trials prop_DeleteUnion 
 (*! QuickProp test_prop_DeleteUnion. *)
 
 Definition prop_UnionDeleteInsert :=
-	ForAll "t " (fun tt => arbitrary) (fun tt t => fuzz t) (fun tt => shrink) (fun tt => show) (
-	Implies (Tree · ∅) "isBST t" (fun '(t, tt) => isBST t) (
-	ForAll "t'" (fun tt => arbitrary) (fun tt t' => fuzz t') (fun tt => shrink) (fun tt => show) (
-	Implies (Tree · _) "isBST t'" (fun '(t', _) => isBST t') (
+	ForAll "t " (fun tt => arbitrary) (fun tt => fuzz) (fun tt => shrink) (fun tt => show) (
+	Implies (Tree · ∅) (fun '(t, tt) => isBST t) (
+	ForAll "t'" (fun tt => arbitrary) (fun tt => fuzz) (fun tt => shrink) (fun tt => show) (
+	Implies (Tree · _) (fun '(t', _) => isBST t') (
 	ForAll "k" (fun tt => arbitrary) (fun tt k => arbitrary) (fun tt => shrink) (fun tt => show) (
 	ForAll "v" (fun tt => arbitrary) (fun tt v => arbitrary) (fun tt => shrink) (fun tt => show) (
 	Check (nat · (nat · (Tree · (Tree · ∅))))
@@ -226,8 +217,8 @@ Definition test_prop_UnionDeleteInsert := (fuzzLoop number_of_trials prop_UnionD
 (*! QuickProp test_prop_UnionDeleteInsert. *)
 
 Definition prop_UnionUnionIdem :=
-	ForAll "t" (fun tt => arbitrary) (fun tt t => fuzz t) (fun tt => shrink) (fun tt => show) (
-	Implies (Tree · ∅) "isBST t" (fun '(t, tt) => isBST t) (
+	ForAll "t" (fun tt => arbitrary) (fun tt => fuzz) (fun tt => shrink) (fun tt => show) (
+	Implies (Tree · ∅) (fun '(t, tt) => isBST t) (
 	Check (Tree · ∅)
 	(fun '(t, tt) => (union t t =|= t)))).
 
@@ -235,12 +226,12 @@ Definition test_prop_UnionUnionIdem := (fuzzLoop number_of_trials prop_UnionUnio
 (*! QuickProp test_prop_UnionUnionIdem. *)
 
 Definition prop_UnionUnionAssoc :=
-	ForAll "t1" (fun tt => arbitrary) (fun tt t1 => fuzz t1) (fun tt => shrink) (fun tt => show) (
-	Implies (Tree · ∅) "isBST t1" (fun '(t1, tt) => isBST t1) (
-	ForAll "t2" (fun tt => arbitrary) (fun tt t2 => fuzz t2) (fun tt => shrink) (fun tt => show) (
-	Implies (Tree · _) "isBST t2" (fun '(t2, _) => isBST t2) (
-	ForAll "t3" (fun tt => arbitrary) (fun tt t3 => fuzz t3) (fun tt => shrink) (fun tt => show) (
-	Implies (Tree · _) "isBST t3" (fun '(t3, _) => isBST t3) (
+	ForAll "t1" (fun tt => arbitrary) (fun tt => fuzz) (fun tt => shrink) (fun tt => show) (
+	Implies (Tree · ∅) (fun '(t1, tt) => isBST t1) (
+	ForAll "t2" (fun tt => arbitrary) (fun tt => fuzz) (fun tt => shrink) (fun tt => show) (
+	Implies (Tree · _) (fun '(t2, _) => isBST t2) (
+	ForAll "t3" (fun tt => arbitrary) (fun tt => fuzz) (fun tt => shrink) (fun tt => show) (
+	Implies (Tree · _) (fun '(t3, _) => isBST t3) (
 	Check (Tree · (Tree · (Tree · ∅)))
 	(fun '(t3, (t2, (t1, tt))) => (union (union t1 t2) t3 =|= union t1 (union t2 t3))))))))).
 
