workloads/Coq/RBTProplang/Strategies/BespokeGenerator.v
@@ -75,7 +75,7 @@ Extract Constant number_of_trials => "max_int".
 
 Definition prop_InsertValid :=
 	ForAll "t" (fun tt => bespoke) (fun tt t => bespoke) (fun tt => shrink) (fun tt => show) (
-	Implies (Tree · ∅) "isRBT t" (fun '(t, tt) => isRBT t) (
+	Implies (Tree · ∅) (fun '(t, tt) => isRBT t) (
 	ForAll "k" (fun tt => genZ) (fun tt k => genZ) (fun tt => shrink) (fun tt => show) (
 	ForAll "v" (fun tt => arbitrary) (fun tt v => arbitrary) (fun tt => shrink) (fun tt => show) (
 	Check (Z · (Z · (Tree · ∅)))
@@ -86,7 +86,7 @@ Definition test_prop_InsertValid := (runLoop number_of_trials prop_InsertValid).
 
 Definition prop_DeleteValid :=
 	ForAll "t" (fun tt => bespoke) (fun tt t => bespoke) (fun tt => shrink) (fun tt => show) (
-	Implies (Tree · ∅) "isRBT t" (fun '(t, tt) => isRBT t) (
+	Implies (Tree · ∅) (fun '(t, tt) => isRBT t) (
 	ForAll "k" (fun tt => genZ) (fun tt n => genZ) (fun tt => shrink) (fun tt => show) (
 	Check (Z · (Tree · ∅))
 	(fun '(k, (t, tt)) => (match delete k t with
@@ -99,7 +99,7 @@ Definition test_prop_DeleteValid := (runLoop number_of_trials prop_DeleteValid).
 
 Definition prop_InsertPost :=
 	ForAll "t" (fun tt => bespoke) (fun tt t => bespoke) (fun tt => shrink) (fun tt => show) (
-	Implies (Tree · ∅) "isRBT t" (fun '(t, tt) => isRBT t) (
+	Implies (Tree · ∅) (fun '(t, tt) => isRBT t) (
 	ForAll "k" (fun tt => genZ) (fun tt k => genZ) (fun tt => shrink) (fun tt => show) (
 	ForAll "k'" (fun tt => genZ) (fun tt k' => genZ) (fun tt => shrink) (fun tt => show) (
 	ForAll "v" (fun tt => arbitrary) (fun tt v => arbitrary) (fun tt => shrink) (fun tt => show) (
@@ -113,7 +113,7 @@ Definition test_prop_InsertPost := (runLoop number_of_trials prop_InsertPost).
 
 Definition prop_DeletePost :=
 	ForAll "t" (fun tt => bespoke) (fun tt t => bespoke) (fun tt => shrink) (fun tt => show) (
-	Implies (Tree · ∅) "isRBT t" (fun '(t, tt) => isRBT t) (
+	Implies (Tree · ∅) (fun '(t, tt) => isRBT t) (
 	ForAll "k" (fun tt => genZ) (fun tt t => genZ) (fun tt => shrink) (fun tt => show) (
 	ForAll "k'" (fun tt => genZ) (fun tt n => genZ) (fun tt => shrink) (fun tt => show) (
 	Check (Z · (Z · (Tree · ∅)))
@@ -126,7 +126,7 @@ Definition test_prop_DeletePost := (runLoop number_of_trials prop_DeletePost).
 
 Definition prop_InsertModel :=
 	ForAll "t" (fun tt => bespoke) (fun tt t => bespoke) (fun tt => shrink) (fun tt => show) (
-	Implies (Tree · ∅) "isRBT t" (fun '(t, tt) => isRBT t) (
+	Implies (Tree · ∅) (fun '(t, tt) => isRBT t) (
 	ForAll "k" (fun tt => genZ) (fun tt t => genZ) (fun tt => shrink) (fun tt => show) (
 	ForAll "v" (fun tt => arbitrary) (fun tt n => arbitrary) (fun tt => shrink) (fun tt => show) (
 	Check (Z · (Z · (Tree · ∅)))
@@ -137,7 +137,7 @@ Definition test_prop_InsertModel := (runLoop number_of_trials prop_InsertModel).
 
 Definition prop_DeleteModel :=
 	ForAll "t" (fun tt => bespoke) (fun tt t => bespoke) (fun tt => shrink) (fun tt => show) (
-	Implies (Tree · ∅) "isRBT t" (fun '(t, tt) => isRBT t) (
+	Implies (Tree · ∅) (fun '(t, tt) => isRBT t) (
 	ForAll "k" (fun tt => genZ) (fun tt t => genZ) (fun tt => shrink) (fun tt => show) (
 	Check (Z · (Tree · ∅))
 	(fun '(k, (t, tt)) => ( match delete k t with
@@ -150,7 +150,7 @@ Definition test_prop_DeleteModel := (runLoop number_of_trials prop_DeleteModel).
 
 Definition prop_InsertInsert :=
 	ForAll "t" (fun tt => bespoke) (fun tt t => bespoke) (fun tt => shrink) (fun tt => show) (
-	Implies (Tree · ∅) "isRBT t" (fun '(t, tt) => isRBT t) (
+	Implies (Tree · ∅) (fun '(t, tt) => isRBT t) (
 	ForAll "k" (fun tt => genZ) (fun tt t => genZ) (fun tt => shrink) (fun tt => show) (
 	ForAll "k'" (fun tt => genZ) (fun tt n => genZ) (fun tt => shrink) (fun tt => show) (
 	ForAll "v" (fun tt => arbitrary) (fun tt v => arbitrary) (fun tt => shrink) (fun tt => show) (
@@ -165,7 +165,7 @@ Definition test_prop_InsertInsert := (runLoop number_of_trials prop_InsertInsert
 
 Definition prop_InsertDelete :=
 	ForAll "t" (fun tt => bespoke) (fun tt t => bespoke) (fun tt => shrink) (fun tt => show) (
-	Implies (Tree · ∅) "isRBT t" (fun '(t, tt) => isRBT t) (
+	Implies (Tree · ∅) (fun '(t, tt) => isRBT t) (
 	ForAll "k" (fun tt => genZ) (fun tt k => genZ) (fun tt => shrink) (fun tt => show) (
 	ForAll "k'" (fun tt => genZ) (fun tt k' => genZ) (fun tt => shrink) (fun tt => show) (
 	ForAll "v" (fun tt => arbitrary) (fun tt v => arbitrary) (fun tt => shrink) (fun tt => show) (
@@ -186,7 +186,7 @@ Definition test_prop_InsertDelete := (runLoop number_of_trials prop_InsertDelete
 
 Definition prop_DeleteInsert :=
 	ForAll "t" (fun tt => bespoke) (fun tt t => bespoke) (fun tt => shrink) (fun tt => show) (
-	Implies (Tree · ∅) "isRBT t" (fun '(t, tt) => isRBT t) (
+	Implies (Tree · ∅) (fun '(t, tt) => isRBT t) (
 	ForAll "k" (fun tt => genZ) (fun tt t => genZ) (fun tt => shrink) (fun tt => show) (
 	ForAll "k'" (fun tt => genZ) (fun tt n => genZ) (fun tt => shrink) (fun tt => show) (
 	ForAll "v'" (fun tt => arbitrary) (fun tt v => arbitrary) (fun tt => shrink) (fun tt => show) (
@@ -209,7 +209,7 @@ Definition test_prop_DeleteInsert := (runLoop number_of_trials prop_DeleteInsert
 
 Definition prop_DeleteDelete :=
 	ForAll "t" (fun tt => bespoke) (fun tt t => bespoke) (fun tt => shrink) (fun tt => show) (
-	Implies (Tree · ∅) "isRBT t" (fun '(t, tt) => isRBT t) (
+	Implies (Tree · ∅) (fun '(t, tt) => isRBT t) (
 	ForAll "k" (fun tt => arbitrary) (fun tt t => arbitrary) (fun tt => shrink) (fun tt => show) (
 	ForAll "k'" (fun tt => arbitrary) (fun tt n => arbitrary) (fun tt => shrink) (fun tt => show) (
 	Check (Z · (Z · (Tree · ∅)))
