workloads/Coq/RBTProplang/Strategies/TypeBasedFuzzer.v
@@ -56,7 +56,7 @@ Open Scope Z_scope.
 
 Definition prop_InsertValid :=
 	ForAll "t" (fun tt => arbitrary) (fun tt t => fuzz t) (fun tt => shrink) (fun tt => show) (
-	Implies (Tree · ∅) "isRBT t" (fun '(t, tt) => isRBT t) (
+	Implies (Tree · ∅) (fun '(t, tt) => isRBT t) (
 	ForAll "k" (fun tt => arbitrary) (fun tt k => fuzz k) (fun tt => shrink) (fun tt => show) (
 	ForAll "v" (fun tt => arbitrary) (fun tt v => fuzz v) (fun tt => shrink) (fun tt => show) (
 	Check (Z · (Z · (Tree · ∅)))
@@ -67,7 +67,7 @@ Definition test_prop_InsertValid := (fuzzLoop number_of_trials prop_InsertValid 
 
 Definition prop_DeleteValid :=
 	ForAll "t" (fun tt => arbitrary) (fun tt t => fuzz t) (fun tt => shrink) (fun tt => show) (
-	Implies (Tree · ∅) "isRBT t" (fun '(t, tt) => isRBT t) (
+	Implies (Tree · ∅) (fun '(t, tt) => isRBT t) (
 	ForAll "k" (fun tt => arbitrary) (fun tt k => fuzz k) (fun tt => shrink) (fun tt => show) (
 	Check (Z · (Tree · ∅))
 	(fun '(k, (t, tt)) => (match delete k t with
@@ -80,7 +80,7 @@ Definition test_prop_DeleteValid := (fuzzLoop number_of_trials prop_DeleteValid 
 
 Definition prop_InsertPost :=
 	ForAll "t" (fun tt => arbitrary) (fun tt t => fuzz t) (fun tt => shrink) (fun tt => show) (
-	Implies (Tree · ∅) "isRBT t" (fun '(t, tt) => isRBT t) (
+	Implies (Tree · ∅) (fun '(t, tt) => isRBT t) (
 	ForAll "k" (fun tt => arbitrary) (fun tt k => fuzz k) (fun tt => shrink) (fun tt => show) (
 	ForAll "k'" (fun tt => arbitrary) (fun tt k' => fuzz k') (fun tt => shrink) (fun tt => show) (
 	ForAll "v" (fun tt => arbitrary) (fun tt v => fuzz v) (fun tt => shrink) (fun tt => show) (
@@ -94,7 +94,7 @@ Definition test_prop_InsertPost := (fuzzLoop number_of_trials prop_InsertPost (H
 
 Definition prop_DeletePost :=
 	ForAll "t" (fun tt => arbitrary) (fun tt t => fuzz t) (fun tt => shrink) (fun tt => show) (
-	Implies (Tree · ∅) "isRBT t" (fun '(t, tt) => isRBT t) (
+	Implies (Tree · ∅) (fun '(t, tt) => isRBT t) (
 	ForAll "k" (fun tt => arbitrary) (fun tt k => fuzz k) (fun tt => shrink) (fun tt => show) (
 	ForAll "k'" (fun tt => arbitrary) (fun tt k' => fuzz k') (fun tt => shrink) (fun tt => show) (
 	Check (Z · (Z · (Tree · ∅)))
@@ -107,7 +107,7 @@ Definition test_prop_DeletePost := (fuzzLoop number_of_trials prop_DeletePost (H
 
 Definition prop_InsertModel :=
 	ForAll "t" (fun tt => arbitrary) (fun tt t => fuzz t) (fun tt => shrink) (fun tt => show) (
-	Implies (Tree · ∅) "isRBT t" (fun '(t, tt) => isRBT t) (
+	Implies (Tree · ∅) (fun '(t, tt) => isRBT t) (
 	ForAll "k" (fun tt => arbitrary) (fun tt k => fuzz k) (fun tt => shrink) (fun tt => show) (
 	ForAll "v" (fun tt => arbitrary) (fun tt v => fuzz v) (fun tt => shrink) (fun tt => show) (
 	Check (Z · (Z · (Tree · ∅)))
@@ -118,7 +118,7 @@ Definition test_prop_InsertModel := (fuzzLoop number_of_trials prop_InsertModel 
 
 Definition prop_DeleteModel :=
 	ForAll "t" (fun tt => arbitrary) (fun tt t => fuzz t) (fun tt => shrink) (fun tt => show) (
-	Implies (Tree · ∅) "isRBT t" (fun '(t, tt) => isRBT t) (
+	Implies (Tree · ∅) (fun '(t, tt) => isRBT t) (
 	ForAll "k" (fun tt => arbitrary) (fun tt k => fuzz k) (fun tt => shrink) (fun tt => show) (
 	Check (Z · (Tree · ∅))
 	(fun '(k, (t, tt)) => ( match delete k t with
@@ -131,7 +131,7 @@ Definition test_prop_DeleteModel := (fuzzLoop number_of_trials prop_DeleteModel 
 
 Definition prop_InsertInsert :=
 	ForAll "t" (fun tt => arbitrary) (fun tt t => fuzz t) (fun tt => shrink) (fun tt => show) (
-	Implies (Tree · ∅) "isRBT t" (fun '(t, tt) => isRBT t) (
+	Implies (Tree · ∅) (fun '(t, tt) => isRBT t) (
 	ForAll "k" (fun tt => arbitrary) (fun tt k => fuzz k) (fun tt => shrink) (fun tt => show) (
 	ForAll "k'" (fun tt => arbitrary) (fun tt k' => fuzz k') (fun tt => shrink) (fun tt => show) (
 	ForAll "v" (fun tt => arbitrary) (fun tt v => fuzz v) (fun tt => shrink) (fun tt => show) (
@@ -146,7 +146,7 @@ Definition test_prop_InsertInsert := (fuzzLoop number_of_trials prop_InsertInser
 
 Definition prop_InsertDelete :=
 	ForAll "t" (fun tt => arbitrary) (fun tt t => fuzz t) (fun tt => shrink) (fun tt => show) (
-	Implies (Tree · ∅) "isRBT t" (fun '(t, tt) => isRBT t) (
+	Implies (Tree · ∅) (fun '(t, tt) => isRBT t) (
 	ForAll "k" (fun tt => arbitrary) (fun tt k => fuzz k) (fun tt => shrink) (fun tt => show) (
 	ForAll "k'" (fun tt => arbitrary) (fun tt k' => fuzz k') (fun tt => shrink) (fun tt => show) (
 	ForAll "v" (fun tt => arbitrary) (fun tt v => fuzz v) (fun tt => shrink) (fun tt => show) (
@@ -167,7 +167,7 @@ Definition test_prop_InsertDelete := (fuzzLoop number_of_trials prop_InsertDelet
 
 Definition prop_DeleteInsert :=
 	ForAll "t" (fun tt => arbitrary) (fun tt t => fuzz t) (fun tt => shrink) (fun tt => show) (
-	Implies (Tree · ∅) "isRBT t" (fun '(t, tt) => isRBT t) (
+	Implies (Tree · ∅) (fun '(t, tt) => isRBT t) (
 	ForAll "k" (fun tt => arbitrary) (fun tt k => fuzz k) (fun tt => shrink) (fun tt => show) (
 	ForAll "k'" (fun tt => arbitrary) (fun tt k' => fuzz k') (fun tt => shrink) (fun tt => show) (
 	ForAll "v'" (fun tt => arbitrary) (fun tt v => fuzz v) (fun tt => shrink) (fun tt => show) (
@@ -190,7 +190,7 @@ Definition test_prop_DeleteInsert := (fuzzLoop number_of_trials prop_DeleteInser
 
 Definition prop_DeleteDelete :=
 	ForAll "t" (fun tt => arbitrary) (fun tt t => fuzz t) (fun tt => shrink) (fun tt => show) (
-	Implies (Tree · ∅) "isRBT t" (fun '(t, tt) => isRBT t) (
+	Implies (Tree · ∅) (fun '(t, tt) => isRBT t) (
 	ForAll "k" (fun tt => arbitrary) (fun tt k => fuzz k) (fun tt => shrink) (fun tt => show) (
 	ForAll "k'" (fun tt => arbitrary) (fun tt k' => fuzz k') (fun tt => shrink) (fun tt => show) (
 	Check (Z · (Z · (Tree · ∅)))
