workloads/Coq/RBTProplang/Strategies/TypeBasedGenerator.v
@@ -34,7 +34,7 @@ Extract Constant number_of_trials => "max_int".
 
 Definition prop_InsertValid :=
 	ForAll "t" (fun tt => arbitrary) (fun tt t => arbitrary) (fun tt => shrink) (fun tt => show) (
-	Implies (Tree · ∅) "isRBT t" (fun '(t, tt) => isRBT t) (
+	Implies (Tree · ∅) (fun '(t, tt) => isRBT t) (
 	ForAll "k" (fun tt => arbitrary) (fun tt k => arbitrary) (fun tt => shrink) (fun tt => show) (
 	ForAll "v" (fun tt => arbitrary) (fun tt v => arbitrary) (fun tt => shrink) (fun tt => show) (
 	Check (Z · (Z · (Tree · ∅)))
@@ -45,7 +45,7 @@ Definition test_prop_InsertValid := (runLoop number_of_trials prop_InsertValid).
 
 Definition prop_DeleteValid :=
 	ForAll "t" (fun tt => arbitrary) (fun tt t => arbitrary) (fun tt => shrink) (fun tt => show) (
-	Implies (Tree · ∅) "isRBT t" (fun '(t, tt) => isRBT t) (
+	Implies (Tree · ∅) (fun '(t, tt) => isRBT t) (
 	ForAll "k" (fun tt => arbitrary) (fun tt n => arbitrary) (fun tt => shrink) (fun tt => show) (
 	Check (Z · (Tree · ∅))
 	(fun '(k, (t, tt)) => (match delete k t with
@@ -58,7 +58,7 @@ Definition test_prop_DeleteValid := (runLoop number_of_trials prop_DeleteValid).
 
 Definition prop_InsertPost :=
 	ForAll "t" (fun tt => arbitrary) (fun tt t => arbitrary) (fun tt => shrink) (fun tt => show) (
-	Implies (Tree · ∅) "isRBT t" (fun '(t, tt) => isRBT t) (
+	Implies (Tree · ∅) (fun '(t, tt) => isRBT t) (
 	ForAll "k" (fun tt => arbitrary) (fun tt k => arbitrary) (fun tt => shrink) (fun tt => show) (
 	ForAll "k'" (fun tt => arbitrary) (fun tt k' => arbitrary) (fun tt => shrink) (fun tt => show) (
 	ForAll "v" (fun tt => arbitrary) (fun tt v => arbitrary) (fun tt => shrink) (fun tt => show) (
@@ -72,7 +72,7 @@ Definition test_prop_InsertPost := (runLoop number_of_trials prop_InsertPost).
 
 Definition prop_DeletePost :=
 	ForAll "t" (fun tt => arbitrary) (fun tt t => arbitrary) (fun tt => shrink) (fun tt => show) (
-	Implies (Tree · ∅) "isRBT t" (fun '(t, tt) => isRBT t) (
+	Implies (Tree · ∅) (fun '(t, tt) => isRBT t) (
 	ForAll "k" (fun tt => arbitrary) (fun tt t => arbitrary) (fun tt => shrink) (fun tt => show) (
 	ForAll "k'" (fun tt => arbitrary) (fun tt n => arbitrary) (fun tt => shrink) (fun tt => show) (
 	Check (Z · (Z · (Tree · ∅)))
@@ -85,7 +85,7 @@ Definition test_prop_DeletePost := (runLoop number_of_trials prop_DeletePost).
 
 Definition prop_InsertModel :=
 	ForAll "t" (fun tt => arbitrary) (fun tt t => arbitrary) (fun tt => shrink) (fun tt => show) (
-	Implies (Tree · ∅) "isRBT t" (fun '(t, tt) => isRBT t) (
+	Implies (Tree · ∅) (fun '(t, tt) => isRBT t) (
 	ForAll "k" (fun tt => arbitrary) (fun tt t => arbitrary) (fun tt => shrink) (fun tt => show) (
 	ForAll "v" (fun tt => arbitrary) (fun tt n => arbitrary) (fun tt => shrink) (fun tt => show) (
 	Check (Z · (Z · (Tree · ∅)))
@@ -96,7 +96,7 @@ Definition test_prop_InsertModel := (runLoop number_of_trials prop_InsertModel).
 
 Definition prop_DeleteModel :=
 	ForAll "t" (fun tt => arbitrary) (fun tt t => arbitrary) (fun tt => shrink) (fun tt => show) (
-	Implies (Tree · ∅) "isRBT t" (fun '(t, tt) => isRBT t) (
+	Implies (Tree · ∅) (fun '(t, tt) => isRBT t) (
 	ForAll "k" (fun tt => arbitrary) (fun tt t => arbitrary) (fun tt => shrink) (fun tt => show) (
 	Check (Z · (Tree · ∅))
 	(fun '(k, (t, tt)) => ( match delete k t with
@@ -109,7 +109,7 @@ Definition test_prop_DeleteModel := (runLoop number_of_trials prop_DeleteModel).
 
 Definition prop_InsertInsert :=
 	ForAll "t" (fun tt => arbitrary) (fun tt t => arbitrary) (fun tt => shrink) (fun tt => show) (
-	Implies (Tree · ∅) "isRBT t" (fun '(t, tt) => isRBT t) (
+	Implies (Tree · ∅) (fun '(t, tt) => isRBT t) (
 	ForAll "k" (fun tt => arbitrary) (fun tt t => arbitrary) (fun tt => shrink) (fun tt => show) (
 	ForAll "k'" (fun tt => arbitrary) (fun tt n => arbitrary) (fun tt => shrink) (fun tt => show) (
 	ForAll "v" (fun tt => arbitrary) (fun tt v => arbitrary) (fun tt => shrink) (fun tt => show) (
@@ -124,7 +124,7 @@ Definition test_prop_InsertInsert := (runLoop number_of_trials prop_InsertInsert
 
 Definition prop_InsertDelete :=
 	ForAll "t" (fun tt => arbitrary) (fun tt t => arbitrary) (fun tt => shrink) (fun tt => show) (
-	Implies (Tree · ∅) "isRBT t" (fun '(t, tt) => isRBT t) (
+	Implies (Tree · ∅) (fun '(t, tt) => isRBT t) (
 	ForAll "k" (fun tt => arbitrary) (fun tt k => arbitrary) (fun tt => shrink) (fun tt => show) (
 	ForAll "k'" (fun tt => arbitrary) (fun tt k' => arbitrary) (fun tt => shrink) (fun tt => show) (
 	ForAll "v" (fun tt => arbitrary) (fun tt v => arbitrary) (fun tt => shrink) (fun tt => show) (
@@ -145,7 +145,7 @@ Definition test_prop_InsertDelete := (runLoop number_of_trials prop_InsertDelete
 
 Definition prop_DeleteInsert :=
 	ForAll "t" (fun tt => arbitrary) (fun tt t => arbitrary) (fun tt => shrink) (fun tt => show) (
-	Implies (Tree · ∅) "isRBT t" (fun '(t, tt) => isRBT t) (
+	Implies (Tree · ∅) (fun '(t, tt) => isRBT t) (
 	ForAll "k" (fun tt => arbitrary) (fun tt t => arbitrary) (fun tt => shrink) (fun tt => show) (
 	ForAll "k'" (fun tt => arbitrary) (fun tt n => arbitrary) (fun tt => shrink) (fun tt => show) (
 	ForAll "v'" (fun tt => arbitrary) (fun tt v => arbitrary) (fun tt => shrink) (fun tt => show) (
@@ -168,7 +168,7 @@ Definition test_prop_DeleteInsert := (runLoop number_of_trials prop_DeleteInsert
 
 Definition prop_DeleteDelete :=
 	ForAll "t" (fun tt => arbitrary) (fun tt t => arbitrary) (fun tt => shrink) (fun tt => show) (
-	Implies (Tree · ∅) "isRBT t" (fun '(t, tt) => isRBT t) (
+	Implies (Tree · ∅) (fun '(t, tt) => isRBT t) (
 	ForAll "k" (fun tt => arbitrary) (fun tt t => arbitrary) (fun tt => shrink) (fun tt => show) (
 	ForAll "k'" (fun tt => arbitrary) (fun tt n => arbitrary) (fun tt => shrink) (fun tt => show) (
 	Check (Z · (Z · (Tree · ∅)))
